Unification (#431)
* Added missing lemmas upto lemma 1

* Performed update

* Part of multiparam lemma2

* More work on lemma 2 multi and unification_problem
Well-formedness is good now
Still needs some uniqueness on subs

* Finished lemma2 and lemma5, rewrote lemma1, lots of extra lemmas

* Removed dead code

* Rest of unification

* PR fixes

* Removed unnecessary comment

* Improve the freshness manager, add automatic tactic for function claims

* Finish technical side conditions

* Fix missing \cdots

* Fix parentheses

---------

Co-authored-by: berpeti <peti.ber007@gmail.com>

matching-logic/src/Theories/FOEquality_ProofSystem.v
@@ -195,6 +195,299 @@ Proof.
   { assumption. }
 Defined.
 
+Lemma functional_pattern_defined {Σ : Signature} {syntax : Syntax} :
+  forall Γ φ, theory ⊆ Γ -> well_formed φ ->
+     Γ ⊢ (ex , (φ =ml b0)) ---> ⌈ φ ⌉.
+Proof.
+  intros Γ φ HΓ Wf.
+  toMLGoal. wf_auto2.
+  mlIntro "H0".
+  mlApplyMeta (forall_functional_subst ⌈ b0 ⌉ φ _ HΓ ltac:(wf_auto2)
+  ltac:(wf_auto2) ltac:(wf_auto2) ltac:(wf_auto2)).
+  mlSplitAnd.
+  * mlClear "H0". fromMLGoal. wf_auto2.
+    remember (fresh_evar patt_bott) as x.
+    pose proof (universal_generalization Γ ⌈patt_free_evar x⌉ x AnyReasoning (pile_any _)) 
+      as H1'.
+    cbn in H1'. case_match. 2: congruence. apply H1'. reflexivity.
+    gapply defined_evar.
+    { apply pile_any. }
+    { exact HΓ. }
+  * mlExact "H0".
+Defined.
+
+Lemma membership_equal_equal {Σ : Signature} {syntax : Syntax} :
+  forall Γ φ φ',
+    theory ⊆ Γ -> mu_free φ' ->
+    well_formed φ -> well_formed φ' ->
+    Γ ⊢ (ex , (φ =ml b0))  ->
+    Γ ⊢ (ex , (φ' =ml b0))  ->
+    Γ ⊢ (φ ∈ml φ') =ml (φ =ml φ') .
+Proof.
+  intros Γ φ φ' HΓ Mufree Wf1 Wf2 Func1 Func2.
+  unfold patt_equal at 1.
+
+  toMLGoal. wf_auto2.
+  mlIntro.
+  pose proof (bott_not_defined Γ) as H.
+  use AnyReasoning in H.
+  mlApplyMeta H.
+  fromMLGoal. wf_auto2.
+
+  apply ceil_monotonic; auto.
+  { wf_auto2. }
+
+  toMLGoal. wf_auto2.
+  pose proof (not_not_intro Γ ((φ ∈ml φ' <---> φ =ml φ' ))
+  ltac:(wf_auto2)) as H0.
+  use AnyReasoning in H0.
+  mlApplyMeta H0.
+  mlSplitAnd; mlIntro.
+  * mlApplyMeta membership_imp_equal_meta; auto. mlExactn 0.
+  * mlApplyMeta equal_imp_membership; auto. mlExactn 0.
+    Unshelve.
+    toMLGoal. wf_auto2.
+    (* clear h. *)
+    mlApplyMeta functional_pattern_defined; auto.
+    mlExactMeta Func2.
+Defined.
+
+Lemma funcional_application {Σ : Signature} {syntax : Syntax} Γ t1 t2 :
+  theory ⊆ Γ ->
+  well_formed t1 ->
+  well_formed t2 ->
+  Γ ⊢ (ex , t2 =ml b0) ---> (all , ex , (t1 ⋅ b1)%ml =ml b0) --->
+    ex , (t1 ⋅ t2)%ml =ml b0.
+Proof.
+  intros HΓ wf1 wf2.
+  mlIntro "H".
+  mlDestructEx "H" as x.
+  mlSimpl. cbn. rewrite evar_open_not_occur. wf_auto2.
+  mlIntro "H0".
+  mlSpecialize "H0" with x.
+  mlSimpl. cbn. rewrite evar_open_not_occur. wf_auto2.
+  mlDestructEx "H0" as y.
+  mlSimpl. cbn. rewrite evar_open_not_occur. wf_auto2.
+  mlExists y.
+  mlSimpl. cbn. rewrite evar_open_not_occur. wf_auto2. rewrite evar_open_not_occur. wf_auto2.
+  mlRewriteBy "H" at 1.
+  mlAssumption.
+Defined.
+
+Section nary_functions.
+
+  Context {Σ : Signature} {syntax : Syntax}.
+  Fixpoint nary_function (f : Pattern) (n : nat) :=
+    match n with
+    | 0 => ex , f =ml b0
+    | S n' => all , nary_function (f ⋅ patt_bound_evar (S n')) n'
+    end.
+
+  Definition nary_function_symbol (f : symbols) (n : nat) := nary_function (patt_sym f) n.
+
+  Eval simpl in nary_function patt_bott 3.
+
+  Lemma nary_function_well_formed_positive :
+    forall n φ, well_formed_positive φ -> well_formed_positive (nary_function φ n).
+  Proof.
+    induction n; simpl; intros.
+    wf_auto2.
+    rewrite IHn. wf_auto2. reflexivity.
+  Qed.
+
+  Lemma nary_function_well_formed_closed_mu_aux :
+    forall m n φ, well_formed_closed_mu_aux φ n ->
+      well_formed_closed_mu_aux (nary_function φ m) n.
+  Proof.
+    induction m; simpl; intros.
+    wf_auto2.
+    rewrite IHm. wf_auto2. reflexivity.
+  Qed.
+
+  Lemma nary_function_well_formed_closed_ex_aux_helper :
+    forall m n φ,
+      n > m ->
+      well_formed_closed_ex_aux φ n ->
+      well_formed_closed_ex_aux (nary_function φ m) (n - S m).
+  Proof.
+    induction m; simpl; intros.
+    wf_auto2.
+    specialize (IHm n (φ ⋅ patt_bound_evar (S m)) ltac:(lia)).
+    rewrite Nat.sub_succ_r. rewrite Nat.succ_pred_pos. lia.
+    rewrite IHm. wf_auto2. case_match. lia. lia. reflexivity.
+  Qed.
+
+  Lemma nary_function_well_formed_closed_ex_aux :
+    forall m n φ, well_formed_closed_ex_aux φ n ->
+      well_formed_closed_ex_aux (nary_function φ m) (n - S m).
+  Proof.
+    intros m n. destruct (dec_gt n m).
+    * intros. by apply nary_function_well_formed_closed_ex_aux_helper.
+    * assert (n - S m = 0) by lia. rewrite H0.
+      assert (n ≤ m) by lia. clear H H0.
+      revert n H1. induction m; intros; cbn.
+      - wf_auto2.
+      - do 2 rewrite andb_true_r.
+        replace 1 with (S (S m) - S m) by lia.
+        apply nary_function_well_formed_closed_ex_aux_helper. lia.
+        wf_auto2. case_match. lia. lia.
+  Qed.
+
+  Lemma nary_function_mu_free :
+    forall m φ, mu_free φ -> mu_free (nary_function φ m).
+  Proof.
+    induction m; intros; simpl. wf_auto2.
+    rewrite IHm; wf_auto2.
+  Qed.
+
+  Lemma nary_function_bevar_subst :
+    forall m n φ ψ,
+      (nary_function φ m)^[evar:n↦ψ] =
+      (nary_function φ^[evar: S m + n ↦ ψ] m).
+  Proof.
+    induction m; intros.
+    * by mlSimpl.
+    * simpl nary_function. mlSimpl. rewrite IHm. mlSimpl.
+      f_equal. f_equal.
+      simpl.
+      case_match. 2-3: lia.
+      rewrite -Nat.add_succ_comm. reflexivity.
+  Qed.
+
+  Lemma function_application_many Γ l φ :
+    theory ⊆ Γ ->
+    wf l ->
+    well_formed φ ->
+    mu_free φ ->
+    foldr andb true (map mu_free l) ->
+    Γ ⊢ nary_function φ (length l) --->
+        foldr (fun p acc => (ex , p =ml b0) ---> acc)
+              (ex , foldl patt_app φ l =ml b0) l.
+  Proof.
+    revert φ.
+    induction l; intros φ HΓ Hwfl Hwf HMF1 HMF2; cbn in *. mlIntro. mlAssumption.
+    destruct_and!.
+    opose proof* (IHl (φ ⋅ a) HΓ H2 ltac:(wf_auto2)).
+    { simpl. by rewrite H HMF1. }
+    { assumption. }
+    toMLGoal.
+    {
+      simpl in *. clear Halmost H.
+      repeat apply well_formed_imp. 2-3: wf_auto2.
+      * assert (well_formed_positive (nary_function (φ ⋅ patt_bound_evar (S (length l))) (length l))). {
+          apply nary_function_well_formed_positive. wf_auto2.
+        }
+        assert (well_formed_closed_mu_aux (nary_function (φ ⋅ patt_bound_evar (S (length l))) (length l)) 0). {
+          apply nary_function_well_formed_closed_mu_aux. wf_auto2.
+        }
+        assert (well_formed_closed_ex_aux (nary_function (φ ⋅ patt_bound_evar (S (length l))) (length l)) 1). {
+          replace 1 with (S (S (length l)) - S (length l)) by lia.
+          apply nary_function_well_formed_closed_ex_aux. wf_auto2.
+          case_match; lia.
+        }
+        wf_auto2.
+      * apply wf_foldr with (t := fun p => (ex , p =ml b0)).
+        - remember (fresh_evar (foldl patt_app (φ ⋅ a) l)) as x.
+          pose proof (evar_quantify_well_formed (foldl patt_app (φ ⋅ a) l =ml patt_free_evar x) x).
+          assert (well_formed (foldl patt_app (φ ⋅ a) l =ml patt_free_evar x)). {
+            rewrite foldl_fold_left.
+            apply well_formed_equal. 2: wf_auto2.
+            apply wf_fold_left with (t := id). wf_auto2. by rewrite map_id.
+            clear. intros. wf_auto2.
+          }
+          mlSimpl in H.
+        - apply map_wf. assumption. clear. intros. wf_auto2.
+        - clear. intros. wf_auto2.
+    }
+    mlIntro. mlIntro.
+    mlApplyMeta IHl.
+    2: { assumption. }
+    2: { simpl. by rewrite H HMF1. }
+    opose proof* (forall_functional_subst (nary_function (φ ⋅ patt_bound_evar (S (length l))) (length l)) a Γ HΓ).
+    { apply nary_function_mu_free. wf_auto2. }
+    { assumption. }
+    {
+      replace 1 with (S (S (length l)) - S (length l)) by lia.
+      apply nary_function_well_formed_closed_ex_aux. wf_auto2.
+      case_match; lia.
+    }
+    { apply nary_function_well_formed_closed_mu_aux. wf_auto2. }
+    2: { assumption. }
+    mlAdd H4. mlConj "0" "1" as "3".
+    mlApply "2" in "3".
+    rewrite nary_function_bevar_subst. mlSimpl. simpl.
+    case_match. 1,3: lia.
+    rewrite Nat.add_0_r.
+    rewrite bevar_subst_not_occur. wf_auto2.
+    mlAssumption.
+  Defined.
+
+End nary_functions.
+
+Fixpoint deconstruct_function {Σ : Signature} (pat : Pattern) : option (symbols * list Pattern) :=
+match pat with
+| patt_app t1 t2 => match deconstruct_function t1 with
+                    | Some (f, pats) => Some (f, pats ++ [t2])
+                    | _ => None
+                    end
+| patt_sym s => Some (s, [])
+| _ => None
+end.
+
+Ltac mlSplitAnds :=
+match goal with
+[ |- @of_MLGoal _ (@mkMLGoal _ ?Γ _ (patt_and _ _) _)] =>
+  mlSplitAnd; mlSplitAnds
+| _ => idtac
+end.
+
+Ltac solve_functional_var :=
+lazymatch goal with
+[ |- @of_MLGoal _ (@mkMLGoal _ ?Γ _ (ex, patt_free_evar ?x =ml b0) _)] =>
+  mlExists x;
+  mlSimpl; cbn; try (rewrite bevar_subst_not_occur; wf_auto2);
+  mlReflexivity
+| [ |- _ ] => fail "Not a functional variable claim"
+end.
+
+Ltac solve_functional_symbol :=
+(* TODO: check the shape, this tactic is fragile *)
+  fromMLGoal;
+  gapply hypothesis;
+  try assumption;
+  wf_auto2;
+  set_solver
+.
+
+Ltac solve_functional_step :=
+  lazymatch goal with
+  | [ |- @of_MLGoal _ (@mkMLGoal _ ?Γ _ (ex, ?p =ml patt_bound_evar 0) _)] =>
+    lazymatch eval cbv in (deconstruct_function p) with
+    | Some (?f, ?p::?pats) =>
+      mlApplyMeta (function_application_many Γ (p::pats) (patt_sym f) ltac:(set_solver) ltac:(wf_auto2) ltac:(wf_auto2) ltac:(by simpl) ltac:(by simpl));
+      try mlSplitAnds
+    | Some (?f, []) => solve_functional_symbol
+    | None => fail "Claim does not contain a first function symbol"
+    end
+  | _ => fail "Claim is not shaped as 'ex, <pat> =ml b0'"
+  end.
+
+Ltac solve_functional :=
+  (repeat solve_functional_step); try solve_functional_var; try solve_functional_symbol.
+
+Goal
+  forall {Σ : Signature} {syntax: Syntax} f g one Γ x y,
+    theory ⊆ Γ ->
+    (all, all, all, ex, patt_app (patt_app (patt_app (patt_sym f) b3) b2) b1 =ml b0) ∈ Γ ->
+    (all, ex, patt_app (patt_sym g) b1 =ml b0) ∈ Γ ->
+    (ex , patt_sym one =ml b0) ∈ Γ ->
+  Γ ⊢ ex, (patt_sym f ⋅ patt_free_evar x ⋅ (patt_sym g ⋅ patt_sym one) ⋅ (patt_sym g ⋅ patt_free_evar y))%ml =ml b0.
+Proof.
+  intros * HΓ Hf Hg Hone.
+  toMLGoal. { wf_auto2. }
+  solve_functional.
+Defined.
+
 Theorem exists_functional_subst_meta: ∀ {Σ : Signature} {syntax : Syntax} (Γ : Theory) (φ φ' : Pattern) ,
   Definedness_Syntax.theory ⊆ Γ ->
   mu_free φ ->
